src/Analysis/Instances/Interval/Ivl_Exec.thy
@@ -26,15 +26,10 @@ text \<open>
 
 subsection \<open>Executable transfer function and seeds, generic in the classifier\<close>
 
-definition assume_ivl_st_for ::
-  "(vname => bool) => bexp => ivl resolved_st_q => ivl resolved_st_q" where
-  "assume_ivl_st_for source_global b s =
-    bfilter_ivl_st source_global b True s"
-
-definition assume_not_ivl_st_for ::
-  "(vname => bool) => bexp => ivl resolved_st_q => ivl resolved_st_q" where
-  "assume_not_ivl_st_for source_global b s =
-    bfilter_ivl_st source_global b False s"
+definition branch_ivl_st_for ::
+  "(vname => bool) => bexp => bool => ivl resolved_st_q => ivl resolved_st_q" where
+  "branch_ivl_st_for source_global b pol s =
+    bfilter_ivl_st source_global b pol s"
 
 definition ivl_enter_st_for ::
   "(vname => bool) => vname list => aexp list =>
@@ -55,9 +50,9 @@ fun ivl_tf_st_for ::
   | "ivl_tf_st_for source_global (EA_Random x) s =
        update_resolved_st_q s (location_of source_global x) ivl_top"
   | "ivl_tf_st_for source_global (EA_Assume b) s =
-       assume_ivl_st_for source_global b s"
+       branch_ivl_st_for source_global b True s"
   | "ivl_tf_st_for source_global (EA_AssumeNot b) s =
-       assume_not_ivl_st_for source_global b s"
+       branch_ivl_st_for source_global b False s"
   | "ivl_tf_st_for source_global (EA_Ret None p) s = s"
   | "ivl_tf_st_for source_global (EA_Ret (Some a) p) s =
        update_resolved_st_q s (location_of source_global ret_var)
@@ -186,21 +181,21 @@ text \<open>Guard filters commute totally through the readback
   (\<open>bfilter_ivl_st_commute\<close>), so full input agreement lifts directly --
   no scope side condition is needed, unlike the write-shaped actions above.\<close>
 
-lemma ivl_tf_st_for_assume_agree:
+lemma ivl_tf_st_for_branch_agree:
   assumes agree: "fun_of_resolved_st_q_for gs s_exec = s_abs"
   shows
-    "fun_of_resolved_st_q_for gs (ivl_tf_st_for gs (EA_Assume b) s_exec) =
-      apply_tf (ivl_tf_for gs) (EA_Assume b) s_abs"
+    "fun_of_resolved_st_q_for gs (branch_ivl_st_for gs b pol s_exec) =
+      branch\<^sup># (ivl_tf_for gs) b pol s_abs"
   unfolding agree[symmetric]
-  by (simp add: assume_ivl_st_for_def bfilter_ivl_st_commute ivl_tf_for_def assume_ivl_def)
+  by (simp add: branch_ivl_st_for_def bfilter_ivl_st_commute ivl_tf_for_def)
 
-lemma ivl_tf_st_for_assume_not_agree:
-  assumes agree: "fun_of_resolved_st_q_for gs s_exec = s_abs"
-  shows
-    "fun_of_resolved_st_q_for gs (ivl_tf_st_for gs (EA_AssumeNot b) s_exec) =
-      apply_tf (ivl_tf_for gs) (EA_AssumeNot b) s_abs"
-  unfolding agree[symmetric]
-  by (simp add: assume_not_ivl_st_for_def bfilter_ivl_st_commute ivl_tf_for_def assume_not_ivl_def)
+lemmas ivl_tf_st_for_assume_agree =
+  ivl_tf_st_for_branch_agree[of gs s_exec s_abs b True for gs s_exec s_abs b,
+    unfolded ivl_tf_st_for.simps(4)[symmetric] apply_tf.simps(4)[symmetric]]
+
+lemmas ivl_tf_st_for_assume_not_agree =
+  ivl_tf_st_for_branch_agree[of gs s_exec s_abs b False for gs s_exec s_abs b,
+    unfolded ivl_tf_st_for.simps(5)[symmetric] apply_tf.simps(5)[symmetric]]
 
 text \<open>
   A per-location specialization of the two lemmas above for the single-
@@ -272,7 +267,7 @@ lemma ivl_tf_st_for_assume_var_lit_agree:
     "lookup_resolved_st_q (ivl_tf_st_for gs (EA_Assume (Less (V x) (N n))) s_exec) location =
       apply_tf (ivl_tf_for gs) (EA_Assume (Less (V x) (N n))) s_abs (location_vname location)"
   using ivl_bfilter_st_for_less_var_lit_agree[OF agree location_in canonical x_in, where res = True]
-  by (simp add: assume_ivl_st_for_def ivl_tf_for_def assume_ivl_def)
+  by (simp add: branch_ivl_st_for_def ivl_tf_for_def apply_tf.simps)
 
 lemma ivl_tf_st_for_assume_not_var_lit_agree:
   fixes s_exec :: "ivl resolved_st_q" and s_abs :: "ivl abs_state"
@@ -286,7 +281,7 @@ lemma ivl_tf_st_for_assume_not_var_lit_agree:
     "lookup_resolved_st_q (ivl_tf_st_for gs (EA_AssumeNot (Less (V x) (N n))) s_exec) location =
       apply_tf (ivl_tf_for gs) (EA_AssumeNot (Less (V x) (N n))) s_abs (location_vname location)"
   using ivl_bfilter_st_for_less_var_lit_agree[OF agree location_in canonical x_in, where res = False]
-  by (simp add: assume_not_ivl_st_for_def ivl_tf_for_def assume_not_ivl_def)
+  by (simp add: branch_ivl_st_for_def ivl_tf_for_def apply_tf.simps)
 
 text \<open>
   A one-argument call entry: the bound formal's location gets the evaluated
