src/Analysis/Instances/Mixed/Rel_Order_Domain.thy
@@ -271,11 +271,17 @@ definition dgs_assign_rel :: "vname \<Rightarrow> aexp \<Rightarrow> relc \<Righ
 definition dgs_random_rel :: "vname \<Rightarrow> relc \<Rightarrow> relc \<Rightarrow> relc \<times> relc" where
   "dgs_random_rel x d g = (forget_relc x g, forget_relc x d)"
 
-definition dgs_assume_rel :: "bexp \<Rightarrow> relc \<Rightarrow> relc \<Rightarrow> relc \<times> relc" where
-  "dgs_assume_rel b d g = (g, assume_step b d)"
+text \<open>
+  \<open>assume_step\<close>/\<open>assume_not_step\<close> stay separate, genuinely asymmetric
+  operations (\<open>x < y\<close> vs.\ its mirror \<open>y \<le> x\<close> insert different pairs, not
+  the same formula under a polarity flag); only the interface-level dispatch
+  consolidates into one @{text tf_branch}-shaped operation.
+\<close>
+definition branch_step_rel :: "bexp \<Rightarrow> bool \<Rightarrow> relc \<Rightarrow> relc" where
+  "branch_step_rel b pol d = (if pol then assume_step b d else assume_not_step b d)"
 
-definition dgs_assume_not_rel :: "bexp \<Rightarrow> relc \<Rightarrow> relc \<Rightarrow> relc \<times> relc" where
-  "dgs_assume_not_rel b d g = (g, assume_not_step b d)"
+definition dgs_branch_rel :: "bexp \<Rightarrow> bool \<Rightarrow> relc \<Rightarrow> relc \<Rightarrow> relc \<times> relc" where
+  "dgs_branch_rel b pol d g = (g, branch_step_rel b pol d)"
 
 definition dgs_enter_rel :: "vname list \<Rightarrow> aexp list \<Rightarrow> relc \<Rightarrow> relc \<Rightarrow> relc \<times> relc" where
   "dgs_enter_rel xs es dc g = (top_relc, top_relc)"
@@ -293,8 +299,7 @@ definition rel_order_spec :: "(relc, relc) dg_spec" where
      dgs_nop = dgs_nop_rel,
      dgs_assign = dgs_assign_rel,
      dgs_random = dgs_random_rel,
-     dgs_assume = dgs_assume_rel,
-     dgs_assume_not = dgs_assume_not_rel,
+     dgs_branch = dgs_branch_rel,
      dgs_enter = dgs_enter_rel,
      dgs_combine_env = dgs_combine_env_rel,
      dgs_combine_assign = dgs_combine_assign_rel
@@ -303,11 +308,11 @@ definition rel_order_spec :: "(relc, relc) dg_spec" where
 named_theorems rel_order_simps
 
 declare
-  dgs_assume_not_rel_def [rel_order_simps]
+  dgs_branch_rel_def     [rel_order_simps]
+  branch_step_rel_def    [rel_order_simps]
   dgs_nop_rel_def        [rel_order_simps]
   rel_order_spec_def     [rel_order_simps]
   gammaDG_rel_def        [rel_order_simps]
-  dgs_assume_rel_def     [rel_order_simps]
   dgs_assign_rel_def     [rel_order_simps]
   dgs_random_rel_def     [rel_order_simps]
 
@@ -344,9 +349,9 @@ proof -
     unfolding dgs_random_rel_def gammaDG_rel_def by simp
 qed
 
-lemma dgs_assume_rel_sound[intro]:
+lemma dgs_branch_rel_sound_True[intro]:
   "edge_collect (EA_Assume b) (gammaDG_rel d g) \<subseteq>
-     (case dgs_assume_rel b d g of (g', d') \<Rightarrow> gammaDG_rel d' g')"
+     (case dgs_branch_rel b True d g of (g', d') \<Rightarrow> gammaDG_rel d' g')"
 proof -
   have "edge_collect (EA_Assume b) (gammaDG_rel d g)
       = {s. s \<in> gammaDG_rel d g \<and> bval b s}"
@@ -354,12 +359,12 @@ proof -
   also have "... \<subseteq> gamma_rel (assume_step b d) \<inter> gamma_rel g"
     using assume_step_sound unfolding gammaDG_rel_def by blast
   finally show ?thesis
-    unfolding dgs_assume_rel_def gammaDG_rel_def by simp
+    unfolding dgs_branch_rel_def branch_step_rel_def gammaDG_rel_def by simp
 qed
 
-lemma dgs_assume_not_rel_sound[intro]:
+lemma dgs_branch_rel_sound_False[intro]:
   "edge_collect (EA_AssumeNot b) (gammaDG_rel d g) \<subseteq>
-     (case dgs_assume_not_rel b d g of (g', d') \<Rightarrow> gammaDG_rel d' g')"
+     (case dgs_branch_rel b False d g of (g', d') \<Rightarrow> gammaDG_rel d' g')"
 proof -
   have "edge_collect (EA_AssumeNot b) (gammaDG_rel d g)
       = {s. s \<in> gammaDG_rel d g \<and> \<not> bval b s}"
@@ -367,7 +372,7 @@ proof -
   also have "... \<subseteq> gamma_rel (assume_not_step b d) \<inter> gamma_rel g"
     using assume_not_step_sound unfolding gammaDG_rel_def by blast
   finally show ?thesis
-    unfolding dgs_assume_not_rel_def gammaDG_rel_def by simp
+    unfolding dgs_branch_rel_def branch_step_rel_def gammaDG_rel_def by simp
 qed
 
 lemma dgs_ret_rel_sound[intro]:
