src/Examples/Sign/Exec_Sign_DG_Run.thy
@@ -150,7 +150,7 @@ proof -
     by unfold_locales
        (rule dgEx_reserved
              sign_ex_transfer.tf_sound_assign_for sign_ex_transfer.tf_sound_random_for
-             sign_ex_transfer.tf_sound_assume_for sign_ex_transfer.tf_sound_assume_not_for
+             sign_ex_transfer.tf_sound_branch_for
              sign_ex_transfer.tf_sound_enter_for sign_ex_transfer.tf_sound_combine_for
              sign_tf_st_for_commute[folded fun_of_exec_dg_st_for_def]
              sign_enter_st_for_commute[folded fun_of_exec_dg_st_for_def]
